SplitImpl.i.dfy

Impl/SplitImpl.i.dfy
@@ -27,7 +27,7 @@ module SplitImpl {
 
   import opened NativeTypes
 
-  method computeValidSplitKey(cache: CacheImpl.MutCache, ref: BT.G.Reference,
+  method computeValidSplitKey(shared cache: CacheImpl.LMutCache, ref: BT.G.Reference,
     pivots: PivotTable, lpivot: Key, rpivot: Option<Key>)
   returns (b: bool)
   requires cache.Inv()
@@ -65,30 +65,25 @@ module SplitImpl {
     return true;
   }
 
-  method splitBookkeeping(s: ImplVariables, left_childref: BT.G.Reference,
+  method splitBookkeeping(linear inout s: ImplVariables, left_childref: BT.G.Reference,
     right_childref: BT.G.Reference, parentref: BT.G.Reference, 
     fparent_children: seq<BT.G.Reference>, shared left_child: Node, 
     shared right_child: Node, slot: uint64)
-  requires Inv(s)
+  requires old_s.Inv()
   requires 0 <= slot as int < |fparent_children|
   requires slot as int < MaxNumChildren()
   requires left_child.Inv()
   requires right_child.Inv()
-  requires s.ready
-  requires BookkeepingModel.ChildrenConditions(s.I(), left_child.children)
-  requires BookkeepingModel.ChildrenConditions(s.I(), right_child.children)
-  requires BookkeepingModel.ChildrenConditions(s.I(), Some(fparent_children))
+  requires old_s.ready
+  requires BookkeepingModel.ChildrenConditions(old_s.I(), left_child.children)
+  requires BookkeepingModel.ChildrenConditions(old_s.I(), right_child.children)
+  requires BookkeepingModel.ChildrenConditions(old_s.I(), Some(fparent_children))
   requires |fparent_children| < MaxNumChildren()
-  requires |s.ephemeralIndirectionTable.I().graph| <= IT.MaxSize() - 3
-  modifies s.lru.Repr
-  modifies s.ephemeralIndirectionTable.Repr
-  modifies s.blockAllocator.Repr
+  requires |old_s.ephemeralIndirectionTable.I().graph| <= IT.MaxSize() - 3
+
   ensures s.ready
   ensures s.W()
-  ensures forall o | o in s.lru.Repr :: o in old(s.lru.Repr) || fresh(o)
-  ensures forall o | o in s.ephemeralIndirectionTable.Repr :: o in old(s.ephemeralIndirectionTable.Repr) || fresh(o)
-  ensures forall o | o in s.blockAllocator.Repr :: o in old(s.blockAllocator.Repr) || fresh(o)
-  ensures s.I() == SplitModel.splitBookkeeping(old(s.I()), left_childref, right_childref, 
+  ensures s.I() == SplitModel.splitBookkeeping(old_s.I(), left_childref, right_childref, 
     parentref, fparent_children, left_child.I(), right_child.I(), slot as int)
   {
     SplitModel.reveal_splitBookkeeping();
@@ -97,70 +92,68 @@ module SplitImpl {
     BookkeepingModel.lemmaChildrenConditionsPreservedWriteBookkeeping(s.I(), left_childref, left_child.children, Some(fparent_children));
     BookkeepingModel.lemmaRefInGraphOfWriteBookkeeping(s.I(), left_childref, left_child.children);
 
-    writeBookkeeping(s, left_childref, left_child.children);
+    writeBookkeeping(inout s, left_childref, left_child.children);
 
     BookkeepingModel.lemmaChildrenConditionsPreservedWriteBookkeeping(s.I(), right_childref, right_child.children, Some(fparent_children));
     BookkeepingModel.lemmaRefInGraphOfWriteBookkeeping(s.I(), right_childref, right_child.children);
     BookkeepingModel.lemmaRefInGraphPreservedWriteBookkeeping(s.I(), right_childref, right_child.children, left_childref);
 
-    writeBookkeeping(s, right_childref, right_child.children);
+    writeBookkeeping(inout s, right_childref, right_child.children);
 
     BookkeepingModel.lemmaChildrenConditionsOfReplace1With2(s.I(), fparent_children, slot as int, left_childref, right_childref);
 
     var rep := Replace1with2(fparent_children, left_childref, right_childref, slot);
-    writeBookkeeping(s, parentref, Some(rep));
+    writeBookkeeping(inout s, parentref, Some(rep));
   }
 
-  method splitCacheChanges(s: ImplVariables, left_childref: BT.G.Reference,
+  method splitCacheChanges(linear inout s: ImplVariables, left_childref: BT.G.Reference,
       right_childref: BT.G.Reference, parentref: BT.G.Reference, slot: uint64, 
       num_children_left: uint64, pivot: Key, linear left_child: Node, linear right_child: Node)
-  requires s.ready
-  requires s.W()
-  requires s.cache.ptr(parentref).Some?
-  requires BT.WFNode(s.cache.I()[parentref])
-  requires s.cache.ptr(parentref).value.I().children.Some?
-  requires 0 <= slot as int < |s.cache.ptr(parentref).value.I().children.value|
+  requires old_s.ready
+  requires old_s.W()
+  requires old_s.cache.ptr(parentref).Some?
+  requires BT.WFNode(old_s.cache.I()[parentref])
+  requires old_s.cache.ptr(parentref).value.I().children.Some?
+  requires 0 <= slot as int < |old_s.cache.ptr(parentref).value.I().children.value|
   requires left_child.Inv()
   requires right_child.Inv()
-  requires |s.cache.I()| <= 0x10000 - 2
+  requires |old_s.cache.I()| <= 0x10000 - 2
   requires left_childref != parentref
   requires right_childref != parentref
-  requires PivotInsertable(s.cache.I()[parentref].pivotTable, (slot+1) as int, pivot)
-  modifies s.Repr()
+  requires PivotInsertable(old_s.cache.I()[parentref].pivotTable, (slot+1) as int, pivot)
+
   ensures s.W()
-  ensures (forall o | o in s.Repr() :: o in old(s.Repr()) || fresh(o))
-  ensures s.I() == SplitModel.splitCacheChanges(old(s.I()), left_childref, right_childref,
+  ensures s.I() == SplitModel.splitCacheChanges(old_s.I(), left_childref, right_childref,
     parentref, slot as int, num_children_left as int, pivot, left_child.I(), right_child.I())
   ensures s.ready
   {
     SplitModel.reveal_splitCacheChanges();
-    s.cache.Insert(left_childref, left_child);
-    s.cache.Insert(right_childref, right_child);
-    s.cache.SplitParent(parentref, slot as uint64, pivot, left_childref, right_childref);
+    inout s.cache.Insert(left_childref, left_child);
+    inout s.cache.Insert(right_childref, right_child);
+    inout s.cache.SplitParent(parentref, slot as uint64, pivot, left_childref, right_childref);
   }
 
-  method splitDoChanges(s: ImplVariables, linear child: Node, left_childref: BT.G.Reference,
+  method splitDoChanges(linear inout s: ImplVariables, linear child: Node, left_childref: BT.G.Reference,
       right_childref: BT.G.Reference, parentref: BT.G.Reference, fparent_pivots: PivotTable,
       fparent_children: seq<BT.G.Reference>, slot: uint64)
-  requires s.ready
-  requires Inv(s)
+  requires old_s.ready
+  requires old_s.Inv()
   requires child.Inv()
   requires BT.WFNode(child.I())
-  requires s.cache.ptr(parentref).Some?
-  requires BT.WFNode(s.cache.I()[parentref])
-  requires fparent_pivots == s.cache.I()[parentref].pivotTable
-  requires Some(fparent_children) == s.cache.I()[parentref].children
+  requires old_s.cache.ptr(parentref).Some?
+  requires BT.WFNode(old_s.cache.I()[parentref])
+  requires fparent_pivots == old_s.cache.I()[parentref].pivotTable
+  requires Some(fparent_children) == old_s.cache.I()[parentref].children
   requires 0 <= slot as int < |fparent_children|
   requires |fparent_children| < MaxNumChildren()
   requires |child.buckets| >= 2
   requires left_childref != parentref
   requires right_childref != parentref
-  requires BookkeepingModel.ChildrenConditions(s.I(), Some(fparent_children))
-  requires BookkeepingModel.ChildrenConditions(s.I(), child.children)
-  requires |s.ephemeralIndirectionTable.I().graph| <= IT.MaxSize() - 3
-  modifies s.Repr()
-  ensures WellUpdated(s)
-  ensures s.I() == SplitModel.splitDoChanges(old(s.I()), old(child.I()), left_childref,
+  requires BookkeepingModel.ChildrenConditions(old_s.I(), Some(fparent_children))
+  requires BookkeepingModel.ChildrenConditions(old_s.I(), child.children)
+  requires |old_s.ephemeralIndirectionTable.I().graph| <= IT.MaxSize() - 3
+  ensures s.W()
+  ensures s.I() == SplitModel.splitDoChanges(old_s.I(), old(child.I()), left_childref,
     right_childref, parentref, fparent_children, slot as int)
   ensures s.ready
   {
@@ -177,9 +170,9 @@ module SplitImpl {
       linear var left_child := child.SplitChildLeft(num_children_left);
       linear var right_child := child.SplitChildRight(num_children_left);
 
-      splitBookkeeping(s, left_childref, right_childref, parentref,
+      splitBookkeeping(inout s, left_childref, right_childref, parentref,
         fparent_children, left_child, right_child, slot as uint64);
-      splitCacheChanges(s, left_childref, right_childref, parentref,
+      splitCacheChanges(inout s, left_childref, right_childref, parentref,
         slot as uint64, num_children_left as uint64, pivot, left_child, right_child);
     } else {
       print "giving up; split can't run because new pivots will not be strictly sorted";
@@ -187,27 +180,26 @@ module SplitImpl {
     var _ := FreeNode(child);
   }
 
-  method splitChild(s: ImplVariables, parentref: BT.G.Reference, 
+  method splitChild(linear inout s: ImplVariables, parentref: BT.G.Reference, 
     childref: BT.G.Reference, slot: uint64, lbound: Key, ubound: Option<Key>,
     fparent_pivots: PivotTable, fparent_children: Option<seq<BT.G.Reference>>)
-  requires s.ready
-  requires Inv(s)
-  requires s.cache.ptr(childref).Some?
-  requires s.cache.ptr(parentref).Some?
-  requires s.cache.I()[parentref].children.Some?
-  requires fparent_pivots == s.cache.I()[parentref].pivotTable
-  requires fparent_children == s.cache.I()[parentref].children
+  requires old_s.ready
+  requires old_s.Inv()
+  requires old_s.cache.ptr(childref).Some?
+  requires old_s.cache.ptr(parentref).Some?
+  requires old_s.cache.I()[parentref].children.Some?
+  requires fparent_pivots == old_s.cache.I()[parentref].pivotTable
+  requires fparent_children == old_s.cache.I()[parentref].children
   requires 0 <= slot as int < |fparent_children.value|
   requires fparent_children.value[slot] == childref
   requires |fparent_children.value| < MaxNumChildren()
-  requires BT.ValidSplitKey(s.cache.I()[childref], lbound, ubound)
-  requires BookkeepingModel.ChildrenConditions(s.I(), fparent_children)
-  requires BookkeepingModel.ChildrenConditions(s.I(), s.cache.I()[childref].children)
-  requires |s.ephemeralIndirectionTable.I().graph| <= IT.MaxSize() - 3
-  modifies s.Repr()
+  requires BT.ValidSplitKey(old_s.cache.I()[childref], lbound, ubound)
+  requires BookkeepingModel.ChildrenConditions(old_s.I(), fparent_children)
+  requires BookkeepingModel.ChildrenConditions(old_s.I(), old_s.cache.I()[childref].children)
+  requires |old_s.ephemeralIndirectionTable.I().graph| <= IT.MaxSize() - 3
   ensures s.ready
-  ensures WellUpdated(s)
-  ensures s.I() == SplitModel.splitChild(old(s.I()), parentref, childref, slot as int, lbound, ubound)
+  ensures s.W()
+  ensures s.I() == SplitModel.splitChild(old_s.I(), parentref, childref, slot as int, lbound, ubound)
   {
     SplitModel.reveal_splitChild();
 
@@ -239,76 +231,75 @@ module SplitImpl {
           print "giving up; doSplit can't allocate right_childref\n";
           var _ := FreeNode(child);
         } else {
-          splitDoChanges(s, child, left_childref.value, right_childref.value,
+          splitDoChanges(inout s, child, left_childref.value, right_childref.value,
             parentref, fparent_pivots, fparent_children.value, slot as uint64);
         }
       }
     }
   }
 
-  method doSplit(s: ImplVariables, parentref: BT.G.Reference, childref: BT.G.Reference, slot: uint64)
-  requires s.ready
-  requires Inv(s)
-  requires s.cache.ptr(childref).Some?
-  requires s.cache.ptr(parentref).Some?
-  requires childref in s.ephemeralIndirectionTable.I().graph
-  requires parentref in s.ephemeralIndirectionTable.I().graph
-  requires s.cache.I()[parentref].children.Some?
-  requires 0 <= slot as int < |s.cache.I()[parentref].children.value|
-  requires s.cache.I()[parentref].children.value[slot] == childref
-  requires |s.cache.I()[parentref].buckets| <= MaxNumChildren() - 1
-  requires |s.ephemeralIndirectionTable.I().graph| <= IT.MaxSize() - 3
-  modifies s.Repr()
-  ensures WellUpdated(s)
+  method doSplit(linear inout s: ImplVariables, parentref: BT.G.Reference, childref: BT.G.Reference, slot: uint64)
+  requires old_s.ready
+  requires old_s.Inv()
+  requires old_s.cache.ptr(childref).Some?
+  requires old_s.cache.ptr(parentref).Some?
+  requires childref in old_s.ephemeralIndirectionTable.I().graph
+  requires parentref in old_s.ephemeralIndirectionTable.I().graph
+  requires old_s.cache.I()[parentref].children.Some?
+  requires 0 <= slot as int < |old_s.cache.I()[parentref].children.value|
+  requires old_s.cache.I()[parentref].children.value[slot] == childref
+  requires |old_s.cache.I()[parentref].buckets| <= MaxNumChildren() - 1
+  requires |old_s.ephemeralIndirectionTable.I().graph| <= IT.MaxSize() - 3
+  ensures s.W()
   ensures s.ready
-  ensures s.I() == SplitModel.doSplit(old(s.I()), parentref, childref, slot as int);
+  ensures s.I() == SplitModel.doSplit(old_s.I(), parentref, childref, slot as int);
   {
     SplitModel.reveal_doSplit();
+    var b := false;
 
-    if s.frozenIndirectionTable != null {
-      var b := s.frozenIndirectionTable.HasEmptyLoc(parentref);
-      if b {
-        print "giving up; split can't run because frozen isn't written";
-        return;
-      }
+    if s.frozenIndirectionTable.lSome? {
+      b := s.frozenIndirectionTable.value.HasEmptyLoc(parentref);
     }
 
-    ghost var fused_parent := s.cache.I()[parentref];
-    ghost var fused_child := s.cache.I()[childref]; 
-    var fparent_pivots, fparent_children := s.cache.GetNodeInfo(parentref);
-    var fchild_pivots, _ := s.cache.GetNodeInfo(childref);
-
-    var childlbound := KeyspaceImpl.cmp(fchild_pivots[0], fparent_pivots[slot]);
-    var childubound := KeyspaceImpl.cmp(fparent_pivots[slot+1], 
-      fchild_pivots[|fchild_pivots| as uint64 -1]);
-
-    if childlbound > 0 || childubound > 0 {
-      print "giving up; split can't run because splitted keys are not in bound";
-      return;
-    }
-
-    BookkeepingModel.lemmaChildrenConditionsOfNode(s.I(), parentref);
-    BookkeepingModel.lemmaChildrenConditionsOfNode(s.I(), childref);
-
-    var lbound := ComputeGetKey(fparent_pivots, slot);
-    var ubound := None;
-    if fparent_pivots[slot+1].Element? {
-      var ukey := ComputeGetKey(fparent_pivots, slot+1);
-      ubound := Some(ukey);
-    }
-    assert lbound == BT.getlbound(fused_parent, slot as int);
-    assert ubound == BT.getubound(fused_parent, slot as int);
-
-    var childvalid := computeValidSplitKey(s.cache, childref, fchild_pivots, lbound, ubound);
-    var parentvalid := computeValidSplitKey(s.cache, parentref, fparent_pivots, lbound, ubound);
-
-    if childvalid && parentvalid {
-      assert BT.ValidSplitKey(fused_parent, lbound, ubound);
-      assert BT.ValidSplitKey(fused_child, lbound, ubound);
-     
-      splitChild(s, parentref, childref, slot, lbound, ubound, fparent_pivots, fparent_children);
+    if b {
+      print "giving up; split can't run because frozen isn't written";
     } else {
-      print "giving up; split can't run because bounds checking failed";
+      ghost var fused_parent := s.cache.I()[parentref];
+      ghost var fused_child := s.cache.I()[childref]; 
+      var fparent_pivots, fparent_children := s.cache.GetNodeInfo(parentref);
+      var fchild_pivots, _ := s.cache.GetNodeInfo(childref);
+
+      var childlbound := KeyspaceImpl.cmp(fchild_pivots[0], fparent_pivots[slot]);
+      var childubound := KeyspaceImpl.cmp(fparent_pivots[slot+1], 
+        fchild_pivots[|fchild_pivots| as uint64 -1]);
+
+      if childlbound > 0 || childubound > 0 {
+        print "giving up; split can't run because splitted keys are not in bound";
+      } else {
+        BookkeepingModel.lemmaChildrenConditionsOfNode(s.I(), parentref);
+        BookkeepingModel.lemmaChildrenConditionsOfNode(s.I(), childref);
+
+        var lbound := ComputeGetKey(fparent_pivots, slot);
+        var ubound := None;
+        if fparent_pivots[slot+1].Element? {
+          var ukey := ComputeGetKey(fparent_pivots, slot+1);
+          ubound := Some(ukey);
+        }
+        assert lbound == BT.getlbound(fused_parent, slot as int);
+        assert ubound == BT.getubound(fused_parent, slot as int);
+
+        var childvalid := computeValidSplitKey(s.cache, childref, fchild_pivots, lbound, ubound);
+        var parentvalid := computeValidSplitKey(s.cache, parentref, fparent_pivots, lbound, ubound);
+
+        if childvalid && parentvalid {
+          assert BT.ValidSplitKey(fused_parent, lbound, ubound);
+          assert BT.ValidSplitKey(fused_child, lbound, ubound);
+        
+          splitChild(inout s, parentref, childref, slot, lbound, ubound, fparent_pivots, fparent_children);
+        } else {
+          print "giving up; split can't run because bounds checking failed";
+        }
+      }
     }
   }
 }
